LeanStlc/StrongNorm.lean
@@ -8,111 +8,158 @@ open LeanSubst
 namespace StrongNormalizaton
 
   @[simp]
-  def LR : Ty -> (Term -> Prop)
-  | .base => λ t => SNi .nor t
-  | .arrow A B => λ t => ∀ (r : Ren) (v : Term), LR A v -> LR B (t[r] :@ v)
-  | .nat => λ t => ∀ (A : Ty) (z s : Term), LR A z -> LR (A -t> A) s -> LR A (.nrec A z s t)
+  def LR (Γ : List Ty) : Ty -> (Term -> Prop)
+  | .base => λ t => Γ ⊢ t : .base ∧ SnNor t
+  | .arrow A B => λ t => Γ ⊢ t : (A -t> B)
+    ∧ ∀ {r Δ v}, Γ -⟨r⟩> Δ -> LR Δ A v -> LR Δ B (t[r] :@ v)
+  | .nat => λ t => Γ ⊢ t : Ty.nat ∧ SnNor t
 
   @[simp]
-  def GR : List Ty -> (Subst Term -> Prop)
-  | Γ, σ => ∀ x T, Γ[x]? = .some T -> LR T ↑(σ x)
+  def GR : List Ty -> List Ty -> (Subst Term -> Prop)
+  | Γ, Δ, σ => ∀ x T, Γ[x]? = .some T -> LR Δ T ↑(σ x)
 
   @[simp]
-  def SemanticTyping Γ t A := ∀ σ, GR Γ σ -> LR A (t[σ])
+  def SemanticTyping Γ t A := ∀ σ Δ, GR Γ Δ σ -> LR Δ A (t[σ])
 
   notation:170 Γ:170 " ⊨s " t:170 " : " A:170 => SemanticTyping Γ t A
 
-  theorem monotone {A t} (r : Ren) : LR A t -> LR A (t[r]) := by
-    intro h; induction A generalizing t r
-    case _ =>
-      simp at *
-      apply SNi.rename r h
-    case _ A B ih1 ih2 =>
-      simp at *; intro r' v rh
-      replace h := h (r' ∘ r) v rh
-      simp at h; apply h
+  theorem LR.typing : LR Γ A t -> Γ ⊢ t : A := by
+    intro j; induction A generalizing Γ t
+    all_goals simp at j; grind
+
+  theorem LR.monotone (m : Γ -⟨r⟩> Δ) : LR Γ A t -> LR Δ A (t[r]) := by
+    intro h; induction A generalizing Γ Δ t r
+    case base => simp at *; sorry
+    case arrow A B ih1 ih2 =>
+      apply And.intro
+      apply Typing.rename m (typing h)
+      intro r' Δ' v m' lv
+      replace h := h.2 (m' ∘ m) lv
+      simp; exact h
+    case nat => sorry
+
 
   theorem cr {A} :
-    (∀ t, LR A t -> SNi .nor t)
-    ∧ (∀ t, SNi .neu t -> LR A t)
-    ∧ (∀ t t', SNi .red (t, t') -> LR A t' -> LR A t)
+    (∀ t, LR Γ A t -> SnNor t)
+    ∧ (∀ t, SnNeu t -> LR Γ A t)
+    ∧ (∀ t t', SnRed t t' -> LR Γ A t' -> LR Γ A t)
   := by
-    induction A <;> simp at *
-    case _ =>
-      apply And.intro _ _
-      apply SNi.neu
-      apply SNi.red
-    case _ A B ih1 ih2 =>
-      apply And.intro
-      case _ =>
-        intro t h
-        apply @SNi.antirename .nor (t[Ren.to (· + 1)]) (· + 1) _ t rfl
-        apply @SNi.beta_var .nor _ _ _ 0 rfl
-        replace h := h (· + 1) (.var 0) (ih1.2.1 (.var 0) SNi.var); simp at h
-        apply ih2.1 _ h
-      case _ =>
-        apply And.intro
-        case _ =>
-          intro t h r v lr
-          apply ih2.2.1
-          apply SNi.app
-          apply SNi.rename r h
-          apply ih1.1 _ lr
-        case _ =>
-          intro t t' h1 h2 r v lr
-          have lem1 := h2 r v lr
-          apply ih2.2.2 (t[r] :@ v) (t'[r] :@ v) _ lem1
-          replace h1 := SNi.rename r h1; simp at h1
-          apply SNi.step h1
+    sorry
+    -- induction A <;> simp at *
+    -- case _ =>
+    --   apply And.intro _ _
+    --   apply SNi.neu
+    --   apply SNi.red
+    -- case _ A B ih1 ih2 =>
+    --   apply And.intro
+    --   case _ =>
+    --     intro t h
+    --     apply @SNi.antirename .nor (t[Ren.to (· + 1)]) (· + 1) _ t rfl
+    --     apply @SNi.beta_var .nor _ _ _ 0 rfl
+    --     replace h := h (· + 1) (.var 0) (ih1.2.1 (.var 0) SNi.var); simp at h
+    --     apply ih2.1 _ h
+    --   case _ =>
+    --     apply And.intro
+    --     case _ =>
+    --       intro t h r v lr
+    --       apply ih2.2.1
+    --       apply SNi.app
+    --       apply SNi.rename r h
+    --       apply ih1.1 _ lr
+    --     case _ =>
+    --       intro t t' h1 h2 r v lr
+    --       have lem1 := h2 r v lr
+    --       apply ih2.2.2 (t[r] :@ v) (t'[r] :@ v) _ lem1
+    --       replace h1 := SNi.rename r h1; simp at h1
+    --       apply SNi.step h1
 
-  theorem var {A x} : LR A (.var x) := by
-    apply cr.2.1; apply SNi.var
+  theorem LR.var {A x} : LR Γ A (.var x) := by
+    apply cr.2.1; apply SnNeu.var
+
+  theorem LR.nrec_neutral : LR Γ A z -> LR Γ (A -t> A) s -> SnNeu n -> LR Γ A (.nrec A z s n) := by
+    intro h1 h2 h3
+    replace h1 := cr.1 _ h1
+    replace h2 := cr.1 _ h2
+    apply cr.2.1
+    apply SnNeu.nrec h1 h2 h3
+
+  theorem LR.app (flr : LR Γ (A -t> B) f) (alr : LR Γ A a) : LR Γ B (f :@ a) := by
+    sorry
+
+  def LR.nrec (h1 : LR Γ A z) (h2 : LR Γ (A -t> A) s) (j : Γ ⊢ n : Ty.nat) : SnNor n -> LR Γ A (.nrec A z s n)
+  | .lam t => by cases j
+  | .zero => cr.2.2 _ _ SnRed.zero h1
+  | .succ t => cr.2.2 _ _ SnRed.succ (app h2 (nrec h1 h2 (by cases j; grind) t))
+  | .neu t => nrec_neutral h1 h2 t
+  | .red r t' => cr.2.2 _ _ (SnRed.step_nrec r) (LR.nrec h1 h2 sorry t')
 
   theorem fundamental {Γ t A} : Γ ⊢ t : A -> Γ ⊨s t : A := by
     intro j; induction j
     case var Γ T x j =>
-      simp; intro σ h
+      simp; intro σ Δ h
       apply h x T j
     case app Γ A B f a j1 j2 ih1 ih2 =>
-      simp; intro σ h; simp at ih1
-      replace ih1 := ih1 σ h id (a[σ])
+      simp; intro σ Δ h; simp at ih1
+      replace ih1 := (ih1 σ Δ h).2 id (a[σ])
       simp at ih1; apply ih1
-      apply ih2 σ h
+      apply ih2 σ Δ h
     case lam Γ A B t j ih =>
-      simp; intro σ h r v lv
-      have lem : t[.re 0::σ ∘ r ∘ +1][.su v :: +0] = t[.su v::σ ∘ r.to] := by simp
-      apply cr.2.2 _ (t[.su v::σ ∘ r.to])
-      have lem2 := @SNi.beta v A (t[.re 0::σ ∘ r ∘ +1]); simp at lem2
-      apply lem2
-      apply cr.1 _ lv
-      replace ih := ih (.su v :: σ ∘ r.to)
-      apply ih
-      simp; intro x T j2
-      cases x
-      case _ =>
-        simp; simp at j2; subst j2
-        apply lv
-      case _ x =>
-        simp; simp at j2
-        replace h := h x T j2
-        unfold Subst.compose; simp
-        generalize zdef : σ x = z at *
-        cases z <;> simp at *
-        case _ k =>
-          have lem := monotone r h; simp at lem
-          generalize wdef : r k = w at *
-          cases w <;> simp [*]
-        case _ t => apply monotone r h
+      sorry
+      -- simp; intro σ Δ h r v lv
+      -- have lem : t[.re 0::σ ∘ r ∘ +1][.su v :: +0] = t[.su v::σ ∘ r.to] := by simp
+      -- apply cr.2.2 _ (t[.su v::σ ∘ r.to])
+      -- have lem2 := @SnRed.beta v A (t[.re 0::σ ∘ r ∘ +1]); simp at lem2
+      -- apply lem2
+      -- apply cr.1 _ lv
+      -- replace ih := ih (.su v :: σ ∘ r.to) Δ
+      -- apply ih
+      -- simp; intro x T j2
+      -- cases x
+      -- case _ =>
+      --   simp; simp at j2; subst j2
+      --   apply lv
+      -- case _ x =>
+      --   simp; simp at j2
+      --   replace h := h x T j2
+      --   unfold Subst.compose; simp
+      --   generalize zdef : σ x = z at *
+      --   cases z <;> simp at *
+      --   case _ k =>
+      --     have lem := LR.monotone r h; simp at lem
+      --     generalize wdef : r k = w at *
+      --     cases w <;> simp [*]
+      --   case _ t => apply LR.monotone r h
+    case zero =>
+      intro σ Δ h; simp
+      sorry
+      -- apply SnNor.zero
+    case succ Γ n j ih =>
+      intro σ Δ h; simp
+      replace ih := ih σ Δ h; simp at ih
+      sorry
+      -- apply SnNor.succ ih
+    case nrec Γ z A s n j1 j2 j3 ih1 ih2 ih3 =>
+      intro σ Δ h; simp
+      replace ih1 := ih1 σ Δ h
+      replace ih2 := ih2 σ Δ h
+      replace ih3 := ih3 σ Δ h
+      have lem := typing_subst Δ σ j3 (by {
+        intro x T j; cases j; case _ j =>
+        replace h := h x T j
+        apply LR.typing h
+      })
+      apply LR.nrec ih1 ih2 lem
+      apply cr.1 _ ih3
 end StrongNormalizaton
 
-theorem strong_normalization_inductive {Γ t A} : Γ ⊢ t : A -> SNi .nor t := by
+theorem strong_normalization_inductive {Γ t A} : Γ ⊢ t : A -> SnNor t := by
   intro j
-  have lem1 : StrongNormalizaton.GR Γ +0 := by
+  have lem1 : StrongNormalizaton.GR Γ Γ +0 := by
     simp; intro x T h
-    apply StrongNormalizaton.var
-  have lem2 := StrongNormalizaton.fundamental j +0 lem1; simp at lem2
+    apply StrongNormalizaton.LR.var
+  have lem2 := StrongNormalizaton.fundamental j +0 Γ lem1; simp at lem2
   apply StrongNormalizaton.cr.1 _ lem2
 
 theorem strong_normalization {Γ t A} : Γ ⊢ t : A -> SN Red t := by
-  intro j; apply @SNi.sound .nor t
+  intro j; apply SnNor.sound
   apply strong_normalization_inductive j
