LeanStlc/Typing.lean
@@ -4,6 +4,7 @@ import LeanStlc.Term
 
 open LeanSubst
 
+@[grind]
 inductive Typing : List Ty -> Term -> Ty -> Prop where
 | var {Γ T x} :
   Γ[x]? = .some T ->
@@ -28,33 +29,44 @@ inductive Typing : List Ty -> Term -> Ty -> Prop where
 
 notation:170 Γ:170 " ⊢ " t:170 " : " A:170 => Typing Γ t A
 
-theorem typing_renaming_lift {Γ Δ} A {r : Ren} :
-  (∀ x T, Γ ⊢ #x : T -> Δ ⊢ #(r x) : T) ->
-  ∀ x T, (A::Γ) ⊢ #x : T -> (A::Δ) ⊢ #(r.lift x) : T
-:= by
-  intro h x T j
-  simp [Ren.lift]; cases x <;> simp at *
-  case _ =>
-    cases j; case _ j =>
-    apply Typing.var
-    simp at *; subst j; rfl
-  case _ x =>
-    cases j; case _ j =>
-    simp at j; apply Typing.var
-    simp; have lem := h x T (Typing.var j)
-    cases lem; case _ lem =>
-    apply lem
+abbrev TypingRen (r : Ren) (Γ Δ : List Ty) := ∀ {x T}, Γ[x]? = some T -> Δ[r x]? = some T
 
-theorem typing_weaken {Γ t A} Δ (r : Ren) :
+notation:35 Γ:35 " -⟨" r "⟩> " Δ:35 => TypingRen r Γ Δ
+
+abbrev TypingSubst (σ : Subst Term) (Γ Δ : List Ty) := ∀ {x T}, Γ[x]? = some T -> Δ ⊢ σ x : T
+
+notation:35 Γ:35 " -[" σ "]> " Δ:35 => TypingSubst σ Γ Δ
+
+theorem TypingRen.lift {Γ Δ : List Ty} A {r : Ren} : Γ -⟨r⟩> Δ -> A::Γ -⟨r.lift⟩> A::Δ := by
+  intro h x T j
+  cases x <;> simp [Ren.lift] at *
+  exact j; case _ x =>
+  apply h j
+
+theorem TypingRen.comp : X -⟨r1⟩> Y -> Y -⟨r2⟩> Z -> X -⟨r2 ∘ r1⟩> Z := by sorry
+
+infixr:90 " ∘ "  => TypingRen.comp
+
+def Typing.rename (m : Γ -⟨r⟩> Δ) : Γ ⊢ t : A -> Δ ⊢ t[r] : A
+| @var Γ T x h => var (m h)
+| app f a => app (f.rename m) (a.rename m)
+| lam t =>
+  let t' := t.rename m.lift
+  lam (by rw [Ren.to_lift] at t'; exact t')
+| zero => zero
+| succ t => succ (t.rename m)
+| nrec z s n => nrec (z.rename m) (s.rename m) (n.rename m)
+
+theorem Typing.rename_old {Γ t A} Δ (r : Ren) :
   Γ ⊢ t : A ->
-  (∀ x T, Γ ⊢ #x : T -> Δ ⊢ #(r x) : T) ->
+  Γ -⟨r⟩> Δ ->
   Δ ⊢ t[r] : A
 := by
   intro j h
   induction j generalizing Δ r
-  case var j =>
-    apply h _ _
-    apply Typing.var j
+  case var T x j =>
+    replace h := h j
+    simp [Ren.to]; apply Typing.var h
   case app j1 j2 ih1 ih2 =>
     apply Typing.app
     replace ih1 := ih1 _ _ h; simp at ih1
@@ -63,7 +75,7 @@ theorem typing_weaken {Γ t A} Δ (r : Ren) :
     apply ih2
   case lam j ih =>
     apply Typing.lam
-    replace ih := ih _ _ (typing_renaming_lift _ h); simp at ih
+    replace ih := ih _ _ (TypingRen.lift _ h); simp at ih
     rw [Ren.to_lift] at ih; apply ih
   case _ Γ' =>
     apply Typing.zero
@@ -79,68 +91,41 @@ theorem typing_weaken {Γ t A} Δ (r : Ren) :
     case _ =>
       apply ih3; intro x T j1; apply h; apply j1
 
-theorem typing_subst_lift {Γ Δ} A {σ : Subst Term} :
-  (∀ x T, Γ ⊢ #x : T -> Δ ⊢ σ x : T) ->
-  ∀ x T, (A::Γ) ⊢ #x : T -> (A::Δ) ⊢ σ.lift x : T
-:= by
-  intro h x T j
-  cases j; case _ j =>
-  cases x <;> simp at *
-  case _ => subst j; apply Typing.var; simp
-  case _ x =>
-    have h' := h _ _ (Typing.var j)
-    have lem := typing_weaken (A :: Δ) (λ x => x + 1) h' (by {
-      intro x T j2; simp
-      apply Typing.var; simp
-      cases j2; simp [*]
-    }); simp at lem
-    unfold Subst.compose; simp
-    generalize zdef : σ x = z at *
-    cases z <;> simp at *
-    all_goals
-      simp [Term.from_action, Subst.compose] at lem
-      rw [zdef] at lem; simp at lem; apply lem
+theorem TypingSubst.lift {Γ Δ : List Ty} A {σ : Subst Term} : Γ -[σ]> Δ -> A::Γ -[σ.lift]> A::Δ := by
+  sorry
 
-theorem typing_subst {Γ t A} Δ (σ : Subst Term) :
-  Γ ⊢ t : A ->
-  (∀ x T, Γ ⊢ #x : T -> Δ ⊢ σ x : T) ->
-  Δ ⊢ t[σ] : A
-:= by
-  intro j h
-  induction j generalizing Δ σ
-  case var T x j =>
-    replace h := h x T; simp
-    generalize zdef : σ x = z at *
-    cases z <;> simp at *
-    all_goals apply h; apply Typing.var j
-  case app j1 j2 ih1 ih2 =>
-    simp; apply Typing.app
-    apply ih1 _ _ h
-    apply ih2 _ _ h
-  case lam j ih =>
-    simp; apply Typing.lam
-    replace ih := ih _ _ (typing_subst_lift _ h)
-    simp at ih; apply ih
-  case _ ih =>
-    simp
-    apply Typing.zero
-  case _ ih =>
-    apply Typing.succ
-    apply ih; exact h
-  case _ ih1 ih2 ih3 =>
-    simp
-    apply Typing.nrec; apply ih1; exact h; apply ih2; exact h; apply ih3; exact h
+-- theorem typing_subst_lift {Γ Δ} A {σ : Subst Term} :
+--   (∀ x T, Γ ⊢ #x : T -> Δ ⊢ σ x : T) ->
+--   ∀ x T, (A::Γ) ⊢ #x : T -> (A::Δ) ⊢ σ.lift x : T
+-- := by
+--   intro h x T j
+--   cases j; case _ j =>
+--   cases x <;> simp at *
+--   case _ => subst j; apply Typing.var; simp
+--   case _ x =>
+--     have h' := h _ _ (Typing.var j)
+--     have lem := typing_weaken (A :: Δ) (λ x => x + 1) h' (by {
+--       intro x T j2; simp
+--       apply Typing.var; simp
+--       cases j2; simp [*]
+--     }); simp at lem
+--     unfold Subst.compose; simp
+--     generalize zdef : σ x = z at *
+--     cases z <;> simp at *
+--     all_goals
+--       simp [Term.from_action, Subst.compose] at lem
+--       rw [zdef] at lem; simp at lem; apply lem
 
-theorem typing_beta {Γ A B b t} : (A::Γ) ⊢ b : B -> Γ ⊢ t : A -> Γ ⊢ b[.su t::+0] : B := by
+def Typing.subst (m : Γ -[σ]> Δ) : Γ ⊢ t : A -> Δ ⊢ t[σ] : A
+| var h => m h
+| app f a => app (f.subst m) (a.subst m)
+| lam t => lam (t.subst m.lift)
+| zero => zero
+| succ t => succ (t.subst m)
+| nrec z s n => nrec (z.subst m) (s.subst m) (n.subst m)
+
+theorem Typing.beta : (A::Γ) ⊢ b : B -> Γ ⊢ t : A -> Γ ⊢ b[.su t::+0] : B := by
   intro j1 j2
-  apply typing_subst Γ (.su t::+0) j1 (λ x T h => by {
-    simp [Term.from_action]; cases x <;> simp
-    case _ =>
-      cases h; case _ h =>
-      simp at h; subst h
-      apply j2
-    case _ x =>
-      cases h; case _ h =>
-      simp at h
-      apply Typing.var h
-  })
+  apply Typing.subst _ j1
+  intro x T h; cases x
+  all_goals simp at *; grind
